= Radical and Rational Equations (SAT) =
== 2020-02-17 | 2020-02-18 ==
==== [[math|Index]] ====

== Stage 2 ==

=== 8sqrt(P) - 2sqrt(3) = sqrt(3) + 3sqrt(P) ===
8sqrt(P) - 2sqrt(3) - 3sqrt(P) = sqrt(3) - 3sqrt(P)

5sqrt(P) - 2sqrt(3) = sqrt(3)

5sqrt(P) - 2sqrt(3) + 2sqrt(3) = sqrt(3) + 2sqrt(3)

 5sqrt(P) = 3sqrt(3)

(5sqrt[P])/3 = (3sqrt[3])/5

 sqrt(P) = (3sqrt[3])/5

(sqrt[P])^2^ = ([3sqrt{3}]/5)^2^

P = (9*3)/25

*_P = 27/25_*

=== 4P^1/2^ + 5P = 0 ===
4P^1/2^ + 5P = 0

4sqrt(P) = -5P

16*P = 25P^2^

16*P - 25P^2^ = 0

P != P^2^

*_P = 0_*

=== K = sqrt(10 + 3K) - 4 ===

*_if K = 2_*

2 = sqrt(10+3[2]) - 4

2 = sqrt(10+6) - 4

2 = sqrt(16) - 4

2 = 4 - 4

2 != 0

*_if K = -2_*

-2 = sqrt(10+3[-2]) - 4

-2 = sqrt(10-6) - 4

-2 = sqrt(4) - 4

-2 = 2 - 4

*-2 == -2*

*_if K = -3_*

-3 = sqrt(10+3[-3]) - 4

-3 = sqrt(10-9) - 4

-3 = sqrt(1) - 4

-3 = 1 - 4

*-3 == -3*


*_K = 2 & K = 3_*

=== 3 + 5X = sqrt(K + 6X) ===
*_if X = 0_*

3 + 5(0) = sqrt(K + 6[0])

3 = sqrt(K)

3^2^ = K

*_9 = K_*

=== X - 5sqrt(X) + 6 = 0 ===
Values of X

X^2^ - 5X + 36 = 0

*_(X - 4)(X - 9)_*

=== (3X - 2)/(2X - 3) = 7/3 ===
Solution to equation

3(3X - 2) = 7(2X - 3)

9X - 6 = 14X - 21

21 - 6 = 14X - 9X

15 = 5X

*_3 = X_*

=== 15Y - 5sqrt(Y) = 0 ===
Least value of Y

15Y^2^ - 5Y = 0

3Y^2^ = Y

_if Y == 0_

3(0)^2^ = 0

*_0 == 0_*

=== (-7)/(9 - 20P) = 3/4 ===
Value of P

-7(4) = 3(9 - 20P)

-28 = 27 - 60P

-28 - 27 = -60P

-55 = -60P

55 = 60P

11 = 12P

*_11/12 = P_*

=== (-2Z)/(Z - 1) + (3)/(7 + 1) = -3 ===
Find the solution(s)

-2Z(Z + 1) + 3(Z - 1) = -3(Z + 1)(Z - 1)

-2Z^2^ - 2Z + 3Z - 3 = -3(Z^2^ - Z) + (Z - 1)

-2Z^2^ - 2Z + 3Z - 3 = -3(Z^2^ - 1)

-2Z^2^ - 2Z + 3Z - 3 = -3Z^2^ + 3

-2Z^2^ + 3Z^2^ + Z - 3 - 3 = 0

Z^2^ + Z - 6

*_(Z - 2)(Z + 3)_*


== Stage 3 ==
===X - X^1/2^ = X^1/2^ ===
Sum of Answers

X - X^1/2^ = X^1/2^

X - X^1/2^ + X^1/2^ = 0

X - X = 0

*_0 == 0_*

_CHECK_

0 - 0^1/2^ = 0^1/2^

0 - 0 = 0

*_0 == 0_*


==== CORRECTION ====

X - X^1/2^ = X^1/2^

X - 2X^1/2^ = 0

X^1/2^(X^1/2^ - 2) = 0

*_X^1/2^ == 2 / X = 0, X = 4_*

_CHECK_

*_if X = 0_*

0 - 0^1/2^ = 0^1/2^

0 == 0

*_if X = 4_*

4 - 4^1/2^ = 4^1/2^

4 -2 = 2

*_2 == 2_*

*_0 + 4 = 4_*

=== (3Z + 2)/(Z - 2) + (Z - 6)/(3Z - 6) = (6Z - 1)/(2Z - 4) ===

9Z + 6 + Z - 6 = 9Z -(3/2)

9Z + Z + 6 - 6 = 9Z -(3/2)

10Z = 9Z -(3/2)

*_Z = -(3/2)_*

=== sqrt(6X - 6) = X -1 ===
Find product of the answers

6X - 6 = X^2^ - 2X + 1

6X = X^2^ - 2X + 1 + 6

6X = X^2^ - 2X + 7

X^2^ - 2X - 6X + 7

X^2^ - 8X + 7

(X - 1)(X - 7)

*_(-1)(-7) = 7_*

=== Y - sqrt(7Y - 31) = 3 ===
Sum of the solutions

Y - 3 = sqrt(7Y - 31)

(Y - 3)^2^ = - 7Y + 31

Y^2^ - 6Y + 9 = 7Y - 31

Y^2^ + 9 + 31 = 7Y + 6Y

Y^2^ + 40 = 13Y

Y^2^  

=== sqrt(L[L - 5]) = 6 ===
Sum of the solutions

L(L - 5) = 36

L^2^ - 5L = 36

L^2^ - 5L - 36

(L + 4)(L - 9)

*_4 - 9 = -5_*

==== CORRECION ====

(L - 4)(L + 9)

*_(-4) + 9 = 5_*
