= Radical and Rational Equations =
== 2020-03-06 ==
==== [[math|Index]] ====

=== Stage 3 ===

(a^2^ * a^-5^)/(a^-3^ * a^0^) * (a^2^/a^3^)^-4^ = a^x^

(a^2^ * a^-5^)/(a^-3^ * a^0^) * a^2 * -4^/a^3 * -4^ = a^x^

(a^2^ * a^-5^)/(a^-3^ * a^0^) * a^-8^/a^-12^ = a^x^

(a^2^ * a^-5^ * a^-8^)/(a^-3^ * a^0^ * a^-12^) = a^x^

a^2 - 5 - 8^/a^-3 + 0 - 12^ = a^x^

a^-11^/a^-15^ = a^x^

a^-11 - (-15)^ = a^x^

a^-11 + 15^ = a^x^

*_a^4^ = a^x^_*

6^1/2^ + 6^3/2^ 

6^1/2^ + 6^1/2^ * 6^1^

6^1/2^ * (1 + 6^1^)

6^1/2^ * (1 + 6)

6^1/2^ * 7

*_7sqrt(6)_*

if Y = 6

if X = 2

6 = -(2-2)^2^ + 6

6 = -(0)^2^ + 6

*_6 = 6_*

if X = 0

2(X - 5)(X - 3)

(2 * -5) * -3

-10 * -3

30


2(X + 5)(X + 3)

(2 * 5) * 3

10 * 3

30

30 = 30

*_Y Intercept is equal_*

5 - 2sqrt(X) = 7 - 5sqrt(X)

5 - 2sqrt(X) + 5sqrt(X) = 7

5 + 3sqrt(X) = 7

3sqrt(X) = 7 - 5

3sqrt(X) = 2

9(X) = 4

*_X = 4/9_*

sqrt(3P + 13) = P + 3

3P + 13 = P^2^ + 6P + 9

P^2^ + 6P - 3P + 9 - 13

P^2^ + 3P - 4

(P + 4)(P - 1)

*_P = -4_*

X/(X - 2) + X/[(X - 2) * (X - 3)] = 4/(X - 3)

X(X - 3) + X = 4(X - 2)

X^2^ - 3X + X = 4X - 8

X^2^ - 2X = 4X - 8

X^2^ = 4X + 2X - 8

X^2^ = 6X - 8

X^2^ - 6X + 8

(X - 4)(X - 2)

_if X = 4_

4/(4 - 2) + 4/[(4 - 2) * (4 - 3)] = 4/(4 - 3)

4/2 + 4/(2 * 1) = 4/1

2 + 4/2 = 4

2 + 2 = 4

*_4 = 4_*

3K/(K + 4) - 4K/(K - 2) = -5

3K * (K - 2) - 4K * (K + 4) = -5 * (K - 2) * (K + 4)

(3K^2^ - 6K) (-4K^2^ - 16K) = (-5K + 10) * (K + 4)

3K^2^ - 4 K^2^ - 6K - 16K = -5K^2^ - 20K + 10K + 40

-K^2^ - 22K = -5K^2^ + 10K + 40

-K^2^ + 5K^2^ - 22K + 10K - 40

4K^2^ - 12K - 40

K^2^ - 3K - 10

(K - 5)(K + 2)

_if K = -2_

3(-2)/(-2 + 4) - 4(-2)/(-2 - 2) = -5

-6/2 - -8/-4 = -5

-3 + - 8/4 = -5

-3 - 2 = -5

*_-5 = -5_*

_if K = 5_

3(5)/(5 + 4) - 4(5)/(5 - 2) = -5

15/9 - 20/3 = -5

5/3 - 20/3 = -5

-15/3 = -5

*_-5 = -5_*

7X = 13sqrt(X)

7X - 13sqrt(X) = 0

7sqrt(X)sqrt(X) - 13sqrt(X) = 0

sqrt(X)[7sqrt(X) - 13]

if sqrt(X) = 0

then X = 0

7sqrt(X) - 13 = 0

7sqrt(X) = 13

sqrt(X) = 13/7

*_X = 169/49_*

